## 17. Equations of second-order surfaces
1. **Write the equation of a sphere with center at point \( P = (1, 2, 3) \) and radius \( r = 3 \).**
  \[
  (x - 1)^2 + (y - 2)^2 + (z - 3)^2 = 9
  \]
2. **Do the spheres with equations \( x^2 + y^2 + z^2 = 1 \) and \( x^2 + y^2 + z^2 = 2 \) have any common points?**
  - No, the spheres do not have any common points because the distance between their centers (which are both at the origin) is zero, but their radii are different.
3. **What curve in space is formed by the intersection of the sphere \( x^2 + y^2 + z^2 = 1 \) with the sphere \( (x-1)^2 + y^2 + z^2 = 1 \)?**
  - The intersection of these spheres forms a circle.
4. **Write the equation of the tangent plane to the paraboloid \( z = (x-1)^2 + y^2 + 1 \) at point \( P(1, 0, 1) \).**
  \[
  z = 1 + 0(x - 1) + 0(y - 0) = 1
  \]
  Thus, the tangent plane is \( z = 1 \).
## 18. Functions
1. **Draw in a single Geogebra notebook the following functions:**
  - \( f(x) = x^2 \)
  - \( g(x) = \sqrt{x} \)
  - \( h(x) = x + 1 \)
  - \( j(x) = \sin(x) \)
  **Find the value of all the above functions at \( x = 2 \).**
  - \( f(2) = 2^2 = 4 \)
  - \( g(2) = \sqrt{2} \approx 1.414 \)
  - \( h(2) = 2 + 1 = 3 \)
  - \( j(2) = \sin(2) \approx 0.909 \)
2. **Let \( f(x) = 3x - 1 \) and \( g(x) = \sqrt{x} \). Find:**
  - \( f(g(x)) = f(\sqrt{x}) = 3\sqrt{x} - 1 \)
  - \( g(f(x)) = g(3x - 1) = \sqrt{3x - 1} \)
  - \( f(f(x)) = f(3x - 1) = 3(3x - 1) - 1 = 9x - 4 \)
  - \( g(g(x)) = g(\sqrt{x}) = \sqrt{\sqrt{x}} = x^{1/4} \)
3. **Let \( f(x) = e^x \) and \( g(x) = \ln(x) \). Check \( f(g(x)) \) and \( g(f(x)) \). What do you notice?**
  - \( f(g(x)) = e^{\ln(x)} = x \)
  - \( g(f(x)) = \ln(e^x) = x \)
  - These functions are inverses of each other.
4. **We have function \( f = \{(1, 7), (2, 9), (3, 11)\} \). Give the inverse function \( f^{-1} \).**
  - \( f^{-1} = \{(7, 1), (9, 2), (11, 3)\} \)
5. **We have function \( f = \{(1, 7), (2, 7), (3, 11)\} \). Give the inverse function \( f^{-1} \).**
  - This function does not have an inverse because it is not one-to-one (the value 7 is mapped from both 1 and 2).
6. **We have function \( f(x) = x - 1 \). Give the inverse function \( f^{-1} \). Show both functions on the same Geogebra notebook.**
  - \( f^{-1}(x) = x + 1 \)
## 19. Limits of Sequences
1. **Calculate:**
  \[
  \lim_{n \to \infty} \frac{n^2 + 3n}{2n^2 - 2n} = \lim_{n \to \infty} \frac{n^2(1 + \frac{3}{n})}{2n^2(1 - \frac{1}{n})} = \lim_{n \to \infty} \frac{1 + \frac{3}{n}}{2 - \frac{1}{n}} = \frac{1}{2}
  \]
  \[
  \lim_{n \to \infty} \frac{(2n + 3)^3}{n^3 - 1} = \lim_{n \to \infty} \frac{8n^3 + 12n^2 + 18n + 27}{n^3(1 - \frac{1}{n^3})} = \lim_{n \to \infty} \frac{8 + \frac{12}{n} + \frac{18}{n^2} + \frac{27}{n^3}}{1 - \frac{1}{n^3}} = 8
  \]
2. **Prove using the squeeze theorem:**
  \[
  -1 \leq \sin(n) \leq 1 \implies -\frac{1}{n} \leq \frac{\sin(n)}{n} \leq \frac{1}{n}
  \]
  As \( n \to \infty \), \( \frac{1}{n} \to 0 \) and \( -\frac{1}{n} \to 0 \), hence by the squeeze theorem:
  \[
  \lim_{n \to \infty} \frac{\sin(n)}{n} = 0
  \]
3. **Find the limit of the sequence:**
  \[
  a_n = \left(1 + \frac{1}{n}\right)^n \quad \text{(This converges to \( e \))}
  \]
## 20. Limits of Real Functions
1. **Compute:**
  \[
  \lim_{x \to \infty} \frac{x^3 + 2x^2}{x^4 - 3x^3} = \lim_{x \to \infty} \frac{x^3(1 + \frac{2}{x})}{x^4(1 - \frac{3}{x})} = \lim_{x \to \infty} \frac{1 + \frac{2}{x}}{x(1 - \frac{3}{x})} = 0
  \]
2. **Find:**
  \[
  \lim_{x \to 0} \frac{\sin(3x)}{2x + 1} = \frac{\sin(3 \cdot 0)}{2 \cdot 0 + 1} = \frac{0}{1} = 0
  \]
3. **Find the asymptotes of the function:**
  - \( f(x) = \frac{x^2 - 1}{x^2 + 1} \)
    - Horizontal asymptote: \( y = 1 \)
  - \( g(x) = \frac{\sin(x)}{x^2 + 1} \)
    - Horizontal asymptote: \( y = 0 \)
## 21. Derivatives
1. **Compute derivatives of functions:**
  \[
  y(x) = -3x + 3 \implies y'(x) = -3
  \]
  \[
  y(x) = \pi x + \sin(1) \implies y'(x) = \pi
  \]
  \[
  y(x) = 4 + \sin(2) \implies y'(x) = 0
  \]
  \[
  y(x) = 2x^3 - 3x^2 + 8x - 9 \implies y'(x) = 6x^2 - 6x + 8
  \]
  \[
  y(x) = 6x^{1/3} \implies y'(x) = 2x^{-2/3}
  \]
  \[
  y(x) = \sqrt{x} \implies y'(x) = \frac{1}{2\sqrt{x}}
  \]
  \[
  y(x) = \cos(x) + \sin(x) \implies y'(x) = -\sin(x) + \cos(x)
  \]
  \[
  y(x) = 2\sin(x)\cos(x) \implies y'(x) = 2(\cos^2(x) - \sin^2(x))
  \]
  \[